# Computational Techniques Assessed Coursework 7

### Solution 1

1. By the definition of Laplace transformation, we know that

$$
L_{k+1}=\int_{0}^{\infin}e^{-st}f(t;k+1,\theta)dt
$$

​		We also observed the following property of $f$
$$
\begin{align}
f'(t;k+1, \theta)&=\frac{d}{dt}(\frac{t^{k}e^{-\frac{t}{\theta}}}{\theta^{k+1}\Gamma(k+1)})\\
&=\frac{d}{dt}(\frac{t^{k}e^{-\frac{t}{\theta}}}{\theta^{k+1}k\Gamma(k)})\\
&=\frac{kt^{k-1}\cdot e^{-\frac{t}{\theta}}-\frac{1}{\theta}\cdot t^k\cdot e^{-\frac{t}{\theta}}}{\theta^{k+1}\cdot k\cdot \Gamma(k)}\\
&=\frac{1}{\theta}\cdot\frac{t^{k-1}e^{-\frac{t}{\theta}}}{\theta^k\Gamma(k)}-\frac{1}{\theta}\cdot\frac{t^k\cdot e^{-\frac{t}{\theta}}}{\theta^{k+1}\cdot k\cdot \Gamma(k)}\\
&=\frac{1}{\theta}(f(t;k,\theta)-f(t;k+1, \theta))
\end{align}
$$
​		By the nature of Laplace transformation, we know that
$$
\begin{align}
(\mathcal{L}f'(t;k+1, \theta))(s)&=sL_{k+1}(s)-f(0;k+1, \theta)=sL_{k+1}(s)
\end{align}
$$
​		Hence we have
$$
\begin{align}
sL_{k+1}(s)&=\int_{0}^{\infin}\frac{e^{-st}}{\theta}(f(t;k,\theta)-f(t;k+1, \theta))dt\\
sL_{k+1}(s)&=\frac{1}{\theta}(L_k(s)-L_{k+1}(s))\\
\theta sL_{k+1}(s)+L_{k+1}(s)&=L_k(s)\\
L_{k+1}(s)&=\frac{L_k(s)}{1+\theta s}
\end{align}
$$

2. When $k=1$, $L_1(s)=\int_{0}^{\infin}e^{-st}\frac{e^{-\frac{t}{\theta}}}{\theta}dt=\frac{1}{\theta}\int_{0}^{\infin}e^{-t(s+\frac{1}{\theta})}dt=\frac{1}{\theta}\cdot \frac{\theta}{1+s\theta}=\frac{1}{1+\theta s}$

   From 1 we have $L_{k+1}(s)=\frac{L_k(s)}{1+\theta s}$. Hence we have
   $$
   L_k(s)=\frac{L_{k-1}(s)}{1+\theta s}=\frac{1}{1+\theta s}\cdot \frac{L_{k-2}(s)}{1+\theta s}=...=\frac{L_1(s)}{(1+\theta s)^{k-1}}=(\frac{1}{1+\theta s})^k
   $$

### Solution 2

The Laplace transform of $e^{iwt}$ is as follows
$$
\mathcal{L}(s)=\int_{0}^{\infin}e^{-st}e^{iwt}dt=\int_{0}^{\infin}e^{-t(s-iw)}dt=(-\frac{e^{-t(s-iw)}}{s-iw})|^{\infin}_{0}=\frac{1}{s-iw}
$$
By Euler's formula, we know that $e^{iwt}=\cos wt+i\sin wt$

Hence the Laplace transformation of $\cos wt$ and $\sin wt$ are
$$
\begin{align}
(\mathcal{L}\cos wt)(s)+(\mathcal{L}i\sin wt)(s)&=\frac{1}{s-iw}\\
(\mathcal{L}\cos wt)(s)+(\mathcal{L}i\sin wt)(s)&=\frac{s+iw}{(s-iw)(s+iw)}\\
(\mathcal{L}\cos wt)(s)+(\mathcal{L}i\sin wt)(s)&=\frac{s+iw}{s^2+w^2}\\
(\mathcal{L}\cos wt)(s)+(\mathcal{L}i\sin wt)(s)&=\frac{s}{s^2+w^2}+\frac{iw}{s^2+w^2}\\
\end{align}
$$
By taking the real parts we have $(\mathcal{L\cos wt})(s)=\frac{s}{s^2+w^2}$ and by taking the imaginary parts we have $(\mathcal{L\sin wt})(s)=\frac{w}{s^2+w^2}$

### Solution 3

1) Using Laplace transformation we have
$$
\begin{align}
s(\mathcal{L}x)(s)-x(0)&=2(\mathcal{L}x)(s)+(\mathcal{L}y)(s)+\int_{0}^{\infin}e^{-st}e^{-t}dt\\
s(\mathcal{L}y)(s)-y(0)&=4(\mathcal{L}x)(s)-(\mathcal{L}y)(s)
\end{align}
$$
​	In the form of linear system using matrix
$$
\begin{align}
\begin{bmatrix}
s-2 & -1\\
-4 & s+1
\end{bmatrix}\begin{bmatrix}
(\mathcal{L}x)(s)\\(\mathcal{L}y)(s)
\end{bmatrix}&=\begin{bmatrix}
\frac{1}{s+1}\\0
\end{bmatrix}\\

\begin{bmatrix}
(\mathcal{L}x)(s)\\(\mathcal{L}y)(s)
\end{bmatrix}&=\frac{1}{(s-2)(s+1)-4}\begin{bmatrix}
s+1 & 1\\
4 & s-2
\end{bmatrix}\begin{bmatrix}
\frac{1}{s+1}\\0
\end{bmatrix}\\
\begin{bmatrix}
(\mathcal{L}x)(s)\\(\mathcal{L}y)(s)
\end{bmatrix}&=\frac{1}{(s-3)(s+2)}\begin{bmatrix}
1\\\frac{4}{s+1}
\end{bmatrix}\\&=\begin{bmatrix}
\frac{1}{(s-3)(s+2)}\\\frac{4}{(s-3)(s+2)(s+1)}
\end{bmatrix}\\
&=\begin{bmatrix}
\frac{1}{5(s-3)} - \frac{1}{5(s+2)}\\
\frac{1}{5(s-3)}+\frac{4}{5(s+2)}-\frac{1}{s+1}
\end{bmatrix}
\end{align}
$$
​	We can then obtain that $x(t)=\frac{e^{3t}}{5}-\frac{e^{-2t}}{5}$ and $y(t)=\frac{e^{3t}}{5}+\frac{4e^{-2}}{5}-e^{{-t}}$

2a) Taking the Laplace transform directly, we have
$$
\begin{align}
s(\mathcal{L}x')(s)-x'(0)&=-w^2(\mathcal{L}x)(s)\\
s(s(\mathcal{L}x)(s)-x(0))-y_0&=-w^2(\mathcal{L}x)(s)\\
s^2(\mathcal{L}x)(s)-x_0s-y_0&=-w^2(\mathcal{L}x)(s)\\
(\mathcal{L}x)(s)&=\frac{x_0s+y_0}{s^2+w^2}
\end{align}
$$
​	From Problem 2 we know that $x(t)=x_0\cos wt+\frac{y_0}{w}\sin wt$

2b) Take $y(t)=x'(t)$, we have
$$
\begin{align}
y'&=-w^2x\\
y&=x'
\end{align}
$$
​		Then we take the Laplace transform
$$
\begin{align}
s(\mathcal{L}y)(s)-y(0)&=-w^2(\mathcal{L}x)(s)\\
(\mathcal{L}y)(s)&=s(\mathcal{L}x)(s)-x(0)
\end{align}
$$
​		which, in matrix form, is
$$
\begin{align}
\begin{bmatrix}
w^2 & s\\
-s & 1
\end{bmatrix}\begin{bmatrix}
X\\Y
\end{bmatrix}&=\begin{bmatrix}
y_0\\x_0
\end{bmatrix}\\
\begin{bmatrix}
X\\Y
\end{bmatrix}&=\frac{1}{s^2+w^2}
\begin{bmatrix}
1 & -s\\
s & w^2
\end{bmatrix}\begin{bmatrix}
y_0\\x_0
\end{bmatrix}\\
\begin{bmatrix}
X\\Y
\end{bmatrix}&=\begin{bmatrix}
\frac{y_0-x_0s}{s^2+w^2}\\
\frac{y_0s+x_0w^2}{s^2+w^2}
\end{bmatrix}
\end{align}
$$

### Solution 4

1) We will partition the fraction as follows
$$
\frac{s-1}{(s+1)(s-2)}=\frac{a}{s+1}+\frac{b}{s-2}
$$
​	From the left hand side we know that
$$
\begin{align}
as-2a+bs+b&=s-1\\
(a+b)s-2a+b&=s-1\\
\Rightarrow \left\{
\begin{matrix}
a+b=1\\
-2a+b=-1
\end{matrix}
\right.\Rightarrow \left\{
\begin{matrix}
a=\frac{2}{3}\\
b=\frac{1}{3}
\end{matrix}
\right.
\end{align}
$$
​	Hence we have
$$
\frac{s-1}{(s+1)(s-2)}=\frac{2}{3(s+1)}+\frac{1}{3(s-2)}
$$
2) We take the Laplace transform on both sides of the equation
$$
\begin{align}
s(\mathcal{L}y_1)(s)-y_1(0)&=4(\mathcal{L}y_2)(s)+\int_{0}^{\infin}2e^{-t}e^{-st}dt\\
s(\mathcal{L}y_2)(s)-y_2(0)&=(\mathcal{L}y_1)(s)
\end{align}
$$
​	which, in the matrix form, is (notice that $X$ denotes the Laplace transform of $y_1$ and $Y$ denotes the Laplace transform of $y_2$)
$$
\begin{align}
\begin{bmatrix}
s & -4\\
-1 & s
\end{bmatrix}\begin{bmatrix}
X\\Y
\end{bmatrix}&=\begin{bmatrix}
1+\frac{2}{1+s}\\
-0.5
\end{bmatrix}\\
\begin{bmatrix}
X\\Y
\end{bmatrix}&=\frac{1}{s^2-4}\begin{bmatrix}
s & 4\\
1 & s
\end{bmatrix}\begin{bmatrix}
1+\frac{2}{1+s}\\
-0.5
\end{bmatrix}\\
\begin{bmatrix}
X\\Y
\end{bmatrix}&=\frac{1}{(s+2)(s-2)}\begin{bmatrix}
\frac{s^2+s-2}{1+s}\\
-\frac{s^2-s-6}{2(1+s)}
\end{bmatrix}\\
\begin{bmatrix}
X\\Y
\end{bmatrix}&=\frac{1}{(s+2)(s-2)}\begin{bmatrix}
\frac{(s+2)(s-1)}{1+s}\\
-\frac{(s-3)(s+2)}{2(1+s)}
\end{bmatrix}\\
\begin{bmatrix}
X\\Y
\end{bmatrix}&=\begin{bmatrix}
\frac{s-1}{(s-2)(s+1)}\\
-\frac{s-3}{2(s+1)(s-2)}
\end{bmatrix}=\begin{bmatrix}
\frac{1}{3(s-2)}+\frac{2}{3(s+1)}\\
-\frac{1}{2}(\frac{4}{3(s+1)}-\frac{1}{3(s-2)})
\end{bmatrix}
\end{align}
$$
​	We can now calculate the solution as follows
$$
\begin{align}
y_1(t)&=\frac{2e^{-t}}{3}+\frac{e^{2t}}{3}\\
y_2(t)&=-\frac{2e^{-t}}{3}+\frac{e^{2t}}{6}
\end{align}
$$

### Solution 7

a) The Fourier series expansion of the following square wave function is
$$
f^N(x)=\sum_{k=0}^{N}a_ke^{iw_kx}=\sum_{k=0}^{N}a_ke^{\pi kx}=\sum_{k=0}^{N}c_k\cos \pi kx+s_k\sin \pi kx
$$
​	where $c_k$ and $s_k$ can be calculated as follows
$$
\begin{align}
c_k&=\frac{1}{2}\int_{0}^{2}f(x)\cos k\pi x dx\\
&=\frac{1}{2}(\int_{0}^{1}\cos k\pi xdx-\int_{1}^{2}\cos k\pi x dx)\\
&=\frac{\sin k\pi}{k\pi}\\
s_k&=\frac{1}{2}(\int_{0}^{2}f(x)\sin k\pi xdx)\\
&=\frac{1}{2}(\int_{0}^{1}\sin k\pi xdx-\int_{1}^{2}\sin k\pi xdx)\\
&=\frac{2(1-\cos k\pi)}{k\pi}
\end{align}
$$
​	then we calculate the value of $c_k$
$$
c_0=\frac{1}{2}\int_{0}^{2}f(x)dx=0
$$
​	Hence the Fourier series expansion of $f(x)$ is
$$
\begin{align}
f^N(x)&=\sum_{k=1}^{N}\frac{\sin k\pi}{k\pi}\cos k\pi x+\frac{2(1-\cos k\pi)}{k\pi}\sin k\pi x\\
&=\sum_{k=1}^{N}\frac{2\sin k\pi x-2\cos k\pi \sin k\pi x}{k\pi}\\
&=\frac{2}{\pi}\sum_{k=1}^{N}\frac{1}{k}\cdot\sin k\pi x(1-\cos k\pi)
\end{align}
$$
